Move notations and tests to separate files

Syntax.v
@@ -1,10 +1,10 @@
-Require Export Bool Ascii String List FunctionalExtensionality Psatz PeanoNat.
+Require Export Bool Ascii String Fin List FunctionalExtensionality Psatz PeanoNat.
 Require Export bbv.Word Lib.VectorFacts Lib.EclecticLib.
 
 Export Word.Notations.
 Export ListNotations.
 
-Require Import Permutation RecordUpdate.RecordSet.
+Require Import Permutation.
 Require Import ZArith.
 
 Global Set Implicit Arguments.
@@ -1820,7 +1820,7 @@ Definition struct_get_field_index
   (n : nat)
   (get_kind : Fin.t (S n) -> Kind)
   (get_name : Fin.t (S n) -> string)
-  (packet : Expr ty (SyntaxKind (Struct get_kind get_name))) (* CHECK *)
+  (packet : Expr ty (SyntaxKind (Struct get_kind get_name)))
   (name : string)
   :  option (Fin.t (S n))
   := nat_rect
@@ -1846,8 +1846,8 @@ Definition struct_get_field_index
               else F H0)
        n
        (PeanoNat.Nat.lt_succ_diag_r n).
-
-Local Ltac struct_get_field_ltac packet name :=
+(* EXPORTED *)
+(* Local *) Ltac struct_get_field_ltac packet name :=
   let val := eval cbv in (struct_get_field_index packet name) in
       match val with
       | Some ?x => exact (ReadStruct packet x)
@@ -1858,8 +1858,8 @@ Local Ltac struct_get_field_ltac packet name :=
         let newstr := constr:(("major error - struct_get_field_index not reducing " ++ name)%string) in
         fail 0 newstr
       end.
-
-Local Ltac struct_set_field_ltac packet name newval :=
+(* EXPORTED *)
+(* Local *) Ltac struct_set_field_ltac packet name newval :=
   let val := eval cbv in (struct_get_field_index packet name) in
       match val with
       | Some ?x => exact (UpdateStruct packet x newval)
@@ -1871,75 +1871,6 @@ Local Ltac struct_set_field_ltac packet name newval :=
         fail 0 newstr
       end.
 
-(* Complex List Actions *)
-(* CHECK *)
-Fixpoint gatherActions (ty: Kind -> Type) k_in (acts: list (ActionT ty k_in)) k_out
-         (cont: list (Expr ty (SyntaxKind k_in)) -> ActionT ty k_out): ActionT ty k_out :=
-  match acts with
-  | nil => cont nil
-  | x :: xs =>
-    (LetAction x (fun val =>
-                    gatherActions xs (fun vals => cont ((Var ltac:(assumption) (SyntaxKind _) val) :: vals))))
-  end.
-
-(* CHECK *)
-Definition readNames (ty: Kind -> Type) k names := map (fun r => 
-                                                         (ReadReg r (SyntaxKind k) 
-                                                                  (fun tmp => 
-                                                                     (Return (Var ltac:(assumption) (SyntaxKind _) tmp))))) names.
-
-(* CHECK *)
-Definition callNames (ty: Kind -> Type) k names := map (fun r =>
-                                                         (MCall r (Void, k) (Const _ Default) (fun tmp => (Return (Var ltac:(assumption) (SyntaxKind _) tmp))))) names.
-
-(* CHECK *)
-Definition writeNames (ty: Kind -> Type) k namesVals :=
-  map (fun r => 
-         (@WriteReg _ _ (fst r) (SyntaxKind k) (snd r)
-                    (Return (Const ty WO)))) namesVals.
-
-(* Notation for normal mods *)
-
-Inductive ModuleElt :=
-| MERegister (_ : RegInitT)
-| MERegAry (_ : list RegInitT)
-| MERule (_ : Attribute (Action Void))
-| MEMeth (_ : DefMethT).
-
-Inductive InModule :=
-| NilInModule
-| ConsInModule (_ : ModuleElt) (_ : InModule).
-
-Fixpoint makeModule' (im : InModule) :=
-  match im with
-  | NilInModule => (nil, nil, nil)
-  | ConsInModule e i =>
-    let '(iregs, irules, imeths) := makeModule' i in
-    match e with
-    | MERegister mreg => (mreg :: iregs, irules, imeths)
-    | MERegAry mregs => (mregs ++ iregs, irules, imeths)
-    | MERule mrule => (iregs, mrule :: irules, imeths)
-    | MEMeth mmeth => (iregs, irules, mmeth :: imeths)
-    end
-  end.
-
-Definition makeModule (im : InModule) :=
-  let '(regs, rules, meths) := makeModule' im in
-  BaseMod regs rules meths.
-
-Definition makeConst k (c: ConstT k): ConstFullT (SyntaxKind k) := SyntaxConst c.
-
-Fixpoint getOrder (im : InModule) :=
-  match im with
-  | NilInModule => nil
-  | ConsInModule e i =>
-    let rest := getOrder i in
-    match e with
-    | MERule mrule => fst mrule :: rest
-    | MEMeth mmeth => fst mmeth :: rest
-    | _ => rest
-    end
-  end.
 
 Local Ltac constructor_simpl :=
   econstructor; eauto; simpl; unfold not; intros.
@@ -1992,8 +1923,7 @@ Ltac discharge_wf :=
   discharge_DisjKey.
 
 
-
-
+(* NOTATIONS WERE HERE *)
 
 Section Positive.
   Local Open Scope positive_scope.
@@ -2048,368 +1978,6 @@ Definition AddIndicesToNames name idxs := map (fun x => AddIndexToName name x) i
 
 
 
-(* Fin.t helpers *)
-Definition ltO{X} : forall n, n < 0 -> X.
-Proof.
-  refine (fun n p => match (_:False) with end); lia.
-Defined.
-
-Lemma ltSmSn_ltmn : forall {m n},
-  S m < S n -> m < n.
-Proof.
-  intros; lia.
-Qed.
-
-Fixpoint mkFin i n : i < n -> Fin.t n :=
-  match n with
-  | 0 => fun p => ltO p
-  | S m => match i with
-           | 0 => fun _ => Fin.F1
-           | S j => fun p => Fin.FS (mkFin (ltSmSn_ltmn p))
-           end
-  end.
-
-
-
-(* Kami notations *)
-Module Import KamiNotations.
-  (** Notations for Struct **)
-
-  Delimit Scope kami_expr_scope with kami_expr.
-
-  Notation "name :: ty" := (name%string,  ty) (only parsing) : kami_struct_scope.
-  Delimit Scope kami_struct_scope with kami_struct.
-
-  (** Notations for expressions *)
-
-  Notation "k @# ty" := (Expr ty (SyntaxKind k)) (no associativity, at level 98, only parsing).
-  Notation "# v" := (Var ltac:(assumption) (SyntaxKind _) v) (only parsing) : kami_expr_scope.
-  Notation "$ n" := (Const _ (natToWord _ n)): kami_expr_scope.
-  Notation "$$ e" := (Const ltac:(assumption) e) (at level 8, only parsing) : kami_expr_scope.
-
-  Notation "! v" := (UniBool Neg v) (at level 35): kami_expr_scope.
-  Notation "e1 && e2" := (CABool And (e1 :: e2 :: nil)) : kami_expr_scope.
-  Notation "e1 || e2" := (CABool Or (e1 :: e2 :: nil)) : kami_expr_scope.
-  Notation "e1 ^^ e2" := (CABool Xor (e1 :: e2 :: nil)) (at level 50): kami_expr_scope.
-  Notation "~ x" := (UniBit (Inv _) x) : kami_expr_scope.
-
-  Notation "a $[ i : j ]":=
-    ltac:(let aTy := type of a in
-          match aTy with
-          | Expr _ (SyntaxKind ?bv) =>
-            let bvSimpl := eval compute in bv in
-                match bvSimpl with
-                | Bit ?w =>
-                  let middle := eval simpl in (i + 1 - j)%nat in
-                      let top := eval simpl in (w - 1 - i)%nat in
-                          exact (ConstExtract j middle top a)
-                end
-          end) (at level 100, i at level 99, only parsing) : kami_expr_scope.
-
-  Notation "a $#[ i : j ]":=
-    ltac:(let aTy := type of a in
-          match aTy with
-          | Expr _ (SyntaxKind ?bv) =>
-            let bvSimpl := eval compute in bv in
-                match bvSimpl with
-                | Bit ?w =>
-                  let middle := eval simpl in (i + 1 - j)%nat in
-                      let top := eval simpl in (w - 1 - i)%nat in
-                          exact (ConstExtract j middle top (@castBits _ w (j + middle + top) ltac:(abstract (lia || nia)) a))
-                end
-          end) (at level 100, i at level 99, only parsing) : kami_expr_scope.
-
-  Notation "e1 + e2" := (CABit (Add) (e1 :: e2 :: nil)) : kami_expr_scope.
-  Notation "e1 * e2" := (CABit (Mul) (e1 :: e2 :: nil)) : kami_expr_scope.
-  Notation "e1 & e2" := (CABit (Band) (e1 :: e2 :: nil)) (at level 201)
-                        : kami_expr_scope.
-  Notation "e1 | e2" := (CABit (Bor) (e1 :: e2 :: nil)) (at level 201)
-                        : kami_expr_scope.
-  Notation "e1 ^ e2" := (CABit (Bxor) (e1 :: e2 :: nil)) : kami_expr_scope.
-  Infix "-" := (BinBit (Sub _)) : kami_expr_scope.
-  Infix "/" := (BinBit (Div _)) : kami_expr_scope.
-  Infix "%%" := (BinBit (Rem _)) (at level 100): kami_expr_scope.
-  Infix "<<" := (BinBit (Sll _ _)) (at level 100) : kami_expr_scope.
-  Infix ">>" := (BinBit (Srl _ _)) (at level 100) : kami_expr_scope.
-  Infix ">>>" := (BinBit (Sra _ _)) (at level 100) : kami_expr_scope.
-  Notation "{< a , .. , b >}" :=
-    ((BinBit (Concat _ _)) a .. (BinBit (Concat _ _) b (@Const _ (Bit 0) WO)) ..)
-      (at level 100, a at level 99): kami_expr_scope.
-  Notation "{< a , .. , b >}" :=
-    (Word.combine b .. (Word.combine a WO) ..)
-      (at level 100, a at level 99): word_scope.
-
-  Infix "<" := (BinBitBool (LessThan _)) : kami_expr_scope.
-  Notation "x > y" := (BinBitBool (LessThan _) y x) : kami_expr_scope.
-  Notation "x >= y" := (UniBool Neg (BinBitBool (LessThan _) x y)) : kami_expr_scope.
-  Notation "x <= y" := (UniBool Neg (BinBitBool (LessThan _) y x)) : kami_expr_scope.
-  Infix "<s" := (Slt _) : kami_expr_scope.
-  Notation "x >s y" := (Slt _ y x) : kami_expr_scope.
-  Notation "x >=s y" := (UniBool Neg (Slt _ x y)) (at level 100) : kami_expr_scope.
-  Notation "x <=s y" := (UniBool Neg (Slt _ y x)) (at level 100): kami_expr_scope.
-  Infix "==" := Eq (at level 39, no associativity) : kami_expr_scope.
-  Notation "x != y" := (UniBool Neg (Eq x y))
-                         (at level 39, no associativity) : kami_expr_scope.
-  Notation "v @[ idx ] " := (ReadArray v idx) (at level 38) : kami_expr_scope.
-  Notation "v '@[' idx <- val ] " := (UpdateArray v idx val) (at level 38) : kami_expr_scope.
-
-  Notation "s @% f" := ltac:(struct_get_field_ltac s%kami_expr f%string)
-                              (at level 38, only parsing): kami_expr_scope.
-
-  Notation "name ::= value" :=
-    (existT (fun a : Attribute Kind => Expr _ (SyntaxKind (snd a)))
-            (name%string, _) value) (at level 50) : kami_struct_init_scope.
-  Delimit Scope kami_struct_init_scope with struct_init.
-
-  Notation getStructVal ls :=
-    (BuildStruct (fun i => snd (nth_Fin (map (@projT1 _ _) ls) i))
-                 (fun j => fst (nth_Fin (map (@projT1 _ _) ls) j))
-                 (fun k => nth_Fin_map2 (@projT1 _ _) (fun x => Expr _ (SyntaxKind (snd x)))
-                                     ls k (projT2 (nth_Fin ls (Fin.cast k (map_length_red (@projT1 _ _) ls)))))).
-
-  Notation "'STRUCT' { s1 ; .. ; sN }" :=
-    (getStructVal (cons s1%struct_init ..
-                        (cons sN%struct_init nil) ..))
-    : kami_expr_scope.
-
-  Notation "name ::= value" :=
-    (name, value) (only parsing): kami_switch_init_scope.
-  Delimit Scope kami_switch_init_scope with switch_init.
-
-  Notation "s '@%[' f <- v ]" := ltac:(struct_set_field_ltac s f v)
-                                       (at level 38, only parsing): kami_expr_scope.
-
-  Notation "'IF' e1 'then' e2 'else' e3" := (ITE e1 e2 e3) : kami_expr_scope.
-
-  Notation "nkind <[ def ]>" := (@NativeKind nkind def) (at level 100): kami_expr_scope.
-
-  (* One hot switches *)
-  Notation "'Switch' val 'Retn' retK 'With' { s1 ; .. ; sN }" :=
-    (unpack retK (CABit Bor (cons (IF val == fst s1%switch_init then pack (snd s1%switch_init) else $0)%kami_expr ..
-                                  (cons (IF val == fst sN%switch_init then pack (snd sN%switch_init)else $0)%kami_expr nil) ..))):
-      kami_expr_scope.
-
-  Notation "'Switch' val 'Of' inK 'Retn' retK 'With' { s1 ; .. ; sN }" :=
-    (unpack retK (CABit Bor (cons (IF val == ((fst s1%switch_init): inK @# _) then pack (snd s1%switch_init) else $0)%kami_expr ..
-                                  (cons (IF val == ((fst sN%switch_init): inK @# _) then pack (snd sN%switch_init)else $0)%kami_expr nil) ..))):
-      kami_expr_scope.
-
-  (* Notations for Let Expressions *)
-  Notation "'LETE' name <- expr ; cont " :=
-    (LetE expr%kami_expr (fun name => cont))
-      (at level 13, right associativity, name at level 99) : kami_expr_scope.
-  Notation "'LETE' name : t <- expr ; cont " :=
-    (LetE (k' := t) expr%kami_expr (fun name => cont))
-      (at level 13, right associativity, name at level 99) : kami_expr_scope.
-  Notation "'RetE' expr" :=
-    (NormExpr expr%kami_expr) (at level 13) : kami_expr_scope.
-  Notation "'LETC' name <- v ; c " :=
-    (LETE name <- RetE v ; c)%kami_expr
-                            (at level 13, right associativity, name at level 99) : kami_expr_scope.
-  Notation "'LETC' name : t <- v ; c " :=
-    (LETE name : t <- RetE v ; c)%kami_expr
-                                (at level 13, right associativity, name at level 99) : kami_expr_scope.
-  Notation "'SystemE' ls ; c " :=
-    (SysE ls c)%kami_expr (at level 13, right associativity, ls at level 99): kami_expr_scope.
-  Notation "'IfE' cexpr 'then' tact 'else' fact 'as' name ; cont " :=
-    (IfElseE cexpr%kami_expr tact fact (fun name => cont))
-      (at level 14, right associativity) : kami_expr_scope.
-  Notation "'IfE' cexpr 'then' tact 'else' fact ; cont " :=
-    (IfElseE cexpr%kami_expr tact fact (fun _ => cont))
-      (at level 14, right associativity) : kami_expr_scope.
-  Notation "'IfE' cexpr 'then' tact ; cont" :=
-    (IfElseE cexpr%kami_expr tact (RetE (Const _ Default))%kami_expr (fun _ => cont))
-      (at level 14, right associativity) : kami_expr_scope.
-
-
-
-  Notation "k ## ty" := (LetExprSyntax ty k) (no associativity, at level 98, only parsing).
-
-  (** Notations for action *)
-
-  Notation "'Call' meth ( a : argT ) ; cont " :=
-    (MCall meth%string (argT, Void) a%kami_expr (fun _ => cont))
-      (at level 13, right associativity, meth at level 0, a at level 99) : kami_action_scope.
-  Notation "'Call' name : retT <- meth ( a : argT ) ; cont " :=
-    (MCall meth%string (argT, retT) a%kami_expr (fun name => cont))
-      (at level 13, right associativity, name at level 0, meth at level 0, a at level 99) : kami_action_scope.
-  Notation "'Call' meth () ; cont " :=
-    (MCall meth%string (Void, Void) (Const _ Default) (fun _ => cont))
-      (at level 13, right associativity, meth at level 0) : kami_action_scope.
-  Notation "'Call' name : retT <- meth () ; cont " :=
-    (MCall meth%string (Void, retT) (Const _ Default) (fun name => cont))
-      (at level 13, right associativity, name at level 0, meth at level 0) : kami_action_scope.
-  Notation "'LETN' name : fullkind <- expr ; cont " :=
-    (LetExpr (k := fullkind) expr%kami_expr (fun name => cont))
-      (at level 13, right associativity, name at level 99) : kami_action_scope.
-  Notation "'LET' name <- expr ; cont " :=
-    (LetExpr expr%kami_expr (fun name => cont))
-      (at level 13, right associativity, name at level 99) : kami_action_scope.
-  Notation "'LET' name : t <- expr ; cont " :=
-    (LetExpr (k := SyntaxKind t) expr%kami_expr (fun name => cont))
-      (at level 13, right associativity, name at level 99) : kami_action_scope.
-  Notation "'LETA' name <- act ; cont " :=
-    (LetAction act (fun name => cont))
-      (at level 13, right associativity, name at level 99) : kami_action_scope.
-  Notation "'LETA' name : t <- act ; cont " :=
-    (LetAction (k := t) act (fun name => cont))
-      (at level 13, right associativity, name at level 99) : kami_action_scope.
-  Notation "'NondetN' name : fullkind ; cont" :=
-    (ReadNondet fullkind (fun name => cont))
-      (at level 13, right associativity, name at level 99) : kami_action_scope.
-  Notation "'Nondet' name : kind ; cont" :=
-    (ReadNondet (SyntaxKind kind) (fun name => cont))
-      (at level 13, right associativity, name at level 99) : kami_action_scope.
-  Notation "'ReadN' name : fullkind <- reg ; cont " :=
-    (ReadReg reg fullkind (fun name => cont))
-      (at level 13, right associativity, name at level 99) : kami_action_scope.
-  Notation "'Read' name <- reg ; cont" :=
-    (ReadReg reg _ (fun name => cont))
-      (at level 13, right associativity, name at level 99) : kami_action_scope.
-  Notation "'Read' name : kind <- reg ; cont " :=
-    (ReadReg reg (SyntaxKind kind) (fun name => cont))
-      (at level 13, right associativity, name at level 99) : kami_action_scope.
-  Notation "'WriteN' reg : fullkind <- expr ; cont " :=
-    (@WriteReg _ _ reg fullkind expr%kami_expr cont)
-      (at level 13, right associativity, reg at level 99) : kami_action_scope.
-  Notation "'Write' reg <- expr ; cont " :=
-    (WriteReg reg expr%kami_expr cont)
-      (at level 13, right associativity, reg at level 99) : kami_action_scope.
-  Notation "'Write' reg : kind <- expr ; cont " :=
-    (@WriteReg _ _ reg (SyntaxKind kind) expr%kami_expr cont)
-      (at level 13, right associativity, reg at level 99) : kami_action_scope.
-  Notation "'If' cexpr 'then' tact 'else' fact 'as' name ; cont " :=
-    (IfElse cexpr%kami_expr tact fact (fun name => cont))
-      (at level 14, right associativity) : kami_action_scope.
-  Notation "'If' cexpr 'then' tact 'else' fact ; cont " :=
-    (IfElse cexpr%kami_expr tact fact (fun _ => cont))
-      (at level 14, right associativity) : kami_action_scope.
-  Notation "'If' cexpr 'then' tact ; cont" :=
-    (IfElse cexpr%kami_expr tact (Return (Const _ Default)) (fun _ => cont))
-      (at level 14, right associativity) : kami_action_scope.
-  Notation "'System' sysexpr ; cont " :=
-    (Sys sysexpr%kami_expr cont)
-      (at level 13, right associativity) : kami_action_scope.
-  Notation "'Ret' expr" :=
-    (Return expr%kami_expr)%kami_expr (at level 13) : kami_action_scope.
-  Notation "'Retv'" := (Return (Const _ (k := Void) Default)) : kami_action_scope.
-
-  Delimit Scope kami_action_scope with kami_action.
-
-  (* Complex list action notations *)
-  Notation "'GatherActions' actionList 'as' val ; cont" :=
-    (gatherActions actionList (fun val => cont))
-      (at level 13, right associativity, val at level 99) : kami_action_scope.
-
-  Notation "'ReadToList' names 'of' k 'as' val ; cont" :=
-    (gatherActions (readNames _ k names) (fun val => cont))
-      (at level 13, right associativity, val at level 99) : kami_action_scope.
-
-  Notation "'CallToList' names 'of' k 'as' val ; cont" :=
-    (gatherActions (callNames _ k names) (fun val => cont))
-      (at level 13, right associativity, val at level 99): kami_action_scope.
-
-  Notation "'WriteToList' names 'of' k 'using' vals ; cont" :=
-    (gatherActions (@writeNames _ k (List.combine names vals)) (fun _ => cont))
-      (at level 13, right associativity, vals at level 99) : kami_action_scope.
-  Delimit Scope kami_init_scope with kami_init.
-
-  Notation "'ARRAY' { x1 ; .. ; xn }" :=
-    (BuildArray (nth_Fin (cons x1%kami_init .. (cons xn%kami_init nil) ..)))
-    : kami_expr_scope.
-
-  Notation "name ::= value" :=
-    (existT (fun a : Attribute Kind => ConstT (snd a))
-            (name%string, _) value) (at level 50) : kami_struct_initial_scope.
-  Delimit Scope kami_struct_initial_scope with struct_initial.
-
-  Notation getStructConst ls :=
-    (ConstStruct (fun i => snd (nth_Fin (map (@projT1 _ _) ls) i))
-                 (fun j => fst (nth_Fin (map (@projT1 _ _) ls) j))
-                 (fun k => nth_Fin_map2 (@projT1 _ _) (fun x => ConstT (snd x))
-                                     ls k (projT2 (nth_Fin ls (Fin.cast k (map_length_red (@projT1 _ _) ls)))))).
-
-  Delimit Scope kami_scope with kami.
-
-  Notation "'RegisterN' name : type <- init" :=
-    (MERegister (name%string, existT RegInitValT type (Some ((NativeConst init)%kami_init)%word)))
-      (at level 13, name at level 99) : kami_scope.
-
-  Notation "'Register' name : type <- init" :=
-    (MERegister (name%string, existT RegInitValT (SyntaxKind type) (Some (makeConst ((init)%kami_init)%word))))
-      (at level 13, name at level 99) : kami_scope.
-
-  Notation "'RegisterU' name : type" :=
-    (MERegister (name%string, existT RegInitValT (SyntaxKind type) None))
-      (at level 13, name at level 99) : kami_scope.
-
-  Notation "'Method' name () : retT := c" :=
-    (MEMeth (name%string, existT MethodT (Void, retT)
-                                 (fun ty (_: ty Void) => c%kami_action : ActionT ty retT)))
-      (at level 13, name at level 9) : kami_scope.
-
-  Notation "'Method' name ( param : dom ) : retT := c" :=
-    (MEMeth (name%string, existT MethodT (dom, retT)
-                                 (fun ty (param : ty dom) => c%kami_action : ActionT ty retT)))
-      (at level 13, name at level 9, param at level 99) : kami_scope.
-
-  Notation "'Rule' name := c" :=
-    (MERule (name%string, fun ty => (c)%kami_action : ActionT ty Void))
-      (at level 13) : kami_scope.
-
-  Notation "'MODULE' { m1 'with' .. 'with' mN }" :=
-    (makeModule (ConsInModule m1%kami .. (ConsInModule mN%kami NilInModule) ..))
-      (only parsing).
-
-
-  Notation "'MODULE_WF' { m1 'with' .. 'with' mN }" :=
-    {| baseModuleWf := {| baseModule := makeModule (ConsInModule m1%kami .. (ConsInModule mN%kami NilInModule) ..) ;
-                          wfBaseModule := ltac:(discharge_wf) |} ;
-       baseModuleOrd := getOrder (ConsInModule m1%kami .. (ConsInModule mN%kami NilInModule) ..) |}
-      (only parsing).
-
-  Notation "'MOD_WF' { m1 'with' .. 'with' mN }" :=
-    {| modWf := {| module := Base (makeModule (ConsInModule m1%kami .. (ConsInModule mN%kami NilInModule) ..)) ;
-                   wfMod := ltac:(discharge_wf) |} ;
-       modOrd := getOrder (ConsInModule m1%kami .. (ConsInModule mN%kami NilInModule) ..) |}
-      (only parsing).
-
-  Notation "'RegisterVec' name 'using' nums : type <- init" :=
-    (MERegAry (
-         map (fun idx =>
-                (AddIndexToName name idx, existT RegInitValT (SyntaxKind type) (Some (makeConst (init)%kami_init)))
-             ) nums
-    ))
-      (at level 13, name at level 9, nums at level 9) : kami_scope.
-
-
-
-  (* Gallina Record Notations *)
-  Notation "x <| proj  :=  v |>" := (set proj (constructor v) x)
-                                      (at level 12, left associativity).
-  Notation "x <| proj  ::==  f |>" := (set proj f x)
-                                        (at level 12, f at next level, left associativity).
-
-
-  Notation "'STRUCT_TYPE' { s1 ; .. ; sN }" :=
-    (getStruct (cons s1%kami_struct .. (cons sN%kami_struct nil) ..)).
-
-  Notation "'ARRAY_CONST' { x1 ; .. ; xn }" :=
-    (ConstArray (nth_Fin' (cons (x1%kami_init)%word .. (cons (xn%kami_init)%word nil) ..) eq_refl)).
-
-  Notation "'STRUCT_CONST' { s1 ; .. ; sN }" :=
-    (getStructConst (cons (s1%struct_initial)%word ..
-                          (cons (sN%struct_initial)%word nil) ..)).
-
-  Notation "i #: n" := (@mkFin (i)%nat (n)%nat ltac:(lia)) (at level 10, only parsing).
-
-  Notation "'Valid' x" := (STRUCT { "valid" ::= $$ true ; "data" ::= x })%kami_expr
-                                                                         (at level 100, only parsing) : kami_expr_scope.
-
-  Notation "'InvData' x" := (STRUCT { "valid" ::= $$ false ; "data" ::= x })%kami_expr
-                                                                            (at level 100, only parsing) : kami_expr_scope.
-
-End KamiNotations.
 
 
 (* Helper functions for struct - Gallina versions of getters and setters *)
@@ -2431,14 +1999,14 @@ Local Definition struct_get_field_aux
   (n : nat)
   (get_kind : Fin.t (S n) -> Kind)
   (get_name : Fin.t (S n) -> string)
-  (packet : Struct get_kind get_name @# ty)
+  (packet : Expr ty (SyntaxKind (Struct get_kind get_name)))
   (name : string)
-  :  option ({kind : Kind & kind @# ty})
+  :  option ({kind : Kind & Expr ty (SyntaxKind kind)})
   := struct_get_field_index packet name >>-
        fun index
          => Some
               (existT
-                (fun kind : Kind => kind @# ty)
+                (fun kind : Kind => Expr ty (SyntaxKind kind))
                 (get_kind index)
                 (ReadStruct packet index)).
 
@@ -2447,21 +2015,21 @@ Definition struct_get_field
   (n : nat)
   (get_value : Fin.t (S n) -> Kind)
   (get_name : Fin.t (S n) -> string)
-  (packet : Struct get_value get_name @# ty)
+  (packet : Expr ty (SyntaxKind (Struct get_value get_name)))
   (name : string)
   (kind : Kind)
-  :  option (kind @# ty)
+  :  option (Expr ty (SyntaxKind kind))
   := struct_get_field_aux packet name >>-
        sigT_rect
-         (fun _ => option (kind @# ty))
+         (fun _ => option (Expr ty (SyntaxKind kind)))
          (fun field_kind field_value
            => sumbool_rect
-                (fun _ => option (kind @# ty))
+                (fun _ => option (Expr ty (SyntaxKind kind)))
                 (fun H : field_kind = kind
                   => Some (
                        eq_rect
                          field_kind
-                         (fun k => k @# ty)
+                         (fun k => Expr ty (SyntaxKind k))
                          field_value
                          kind
                          H))
@@ -2474,11 +2042,11 @@ Definition struct_get_field_default
   (n : nat)
   (get_value : Fin.t (S n) -> Kind)
   (get_name : Fin.t (S n) -> string)
-  (packet : Struct get_value get_name @# ty)
+  (packet : Expr ty (SyntaxKind (Struct get_value get_name)))
   (name : string)
   (kind : Kind)
-  (default : kind @# ty)
-  :  kind @# ty
+  (default : Expr ty (SyntaxKind kind))
+  :  Expr ty (SyntaxKind kind)
   := match struct_get_field packet name kind with
        | Some field_value
          => field_value
@@ -2491,218 +2059,220 @@ Definition struct_set_field
   (n : nat)
   (get_kind : Fin.t (S n) -> Kind)
   (get_name : Fin.t (S n) -> string)
-  (packet : Struct get_kind get_name @# ty)
+  (packet : Expr ty (SyntaxKind (Struct get_kind get_name)))
   (name : string)
   (kind : Kind)
-  (value : kind @# ty)
-  :  option (Struct get_kind get_name @# ty)
+  (value : Expr ty (SyntaxKind kind))
+  :  option (Expr ty (SyntaxKind (Struct get_kind get_name)))
   := struct_get_field_index packet name >>-
        fun index
          => sumbool_rect
-              (fun _ => option (Struct get_kind get_name @# ty))
+              (fun _ => option (Expr ty (SyntaxKind (Struct get_kind get_name))))
               (fun H : get_kind index = kind
                 => Some
                      (UpdateStruct packet index
-                       (eq_rect_r (fun k => k @# ty) value H)))
+                       (eq_rect_r (fun k => Expr ty (SyntaxKind k)) value H)))
              (fun _ => None)
              (Kind_dec (get_kind index) kind).
 
-
-
-
-
-Section mod_test.
-  Variable a: string.
-  Local Notation "^ x" := (a ++ "." ++ x)%string (at level 0).
-  Local Example test := MOD_WF{
-                              Register (^"x") : Bool <- true
-                                with Register (^"y") : Bool <- false
-                                with Rule (^"r1") := ( Read y: Bool <- ^"y";
-                                                         Write (^"x"): Bool <- #y;
-                                                         Retv )
-                          }.
-
-  Local Example test1 := MODULE_WF{
-                             Register (^"x") : Bool <- true
-                               with Register (^"y") : Bool <- false
-                               with Rule (^"r1") := ( Read y: Bool <- ^"y";
-                                                        Write (^"x"): Bool <- #y;
-                                                        Retv )
-                           }.
-End mod_test.
-
-
-
-
-
-Local Example test_normaldisj:
-  DisjKey (map (fun x => (x, 1)) ("a" :: "b" :: "c" :: nil))%string
-          (map (fun x => (x, 2)) ("d" :: "e" :: nil))%string.
-Proof.
-  simpl.
-  discharge_DisjKey.
-Qed.
-
-Local Example test_prefix_disj a:
-  DisjKey (map (fun x => ((a ++ x)%string, 1)) ("ab" :: "be" :: "cs" :: nil))%string
-          (map (fun x => ((a ++ x)%string, 2)) ("de" :: "et" :: nil))%string.
-Proof.
-  simpl.
-  discharge_DisjKey.
-Qed.
-
-Local Example test_suffix_disj a:
-  DisjKey (map (fun x => ((x ++ a)%string, 1)) ("ab" :: "be" :: "cs" :: nil))%string
-          (map (fun x => ((x ++ a)%string, 2)) ("de" :: "et" :: nil))%string.
-Proof.
-  simpl.
-  discharge_DisjKey.
-Qed.
-
-
-
-
-
-
-(* Testing the Notations *)
-
-Local Example testSwitch ty (val: Bit 5 @# ty) (a b: Bool @# ty) : Bool @# ty :=
-  (Switch val Retn Bool With {
-            $$ (natToWord 5 5) ::= $$ true ;
-            $$ (natToWord 5 6) ::= $$ false
-          })%kami_expr.
-
-Local Example testSwitch2 ty (val: Bit 5 @# ty) (a b: Bool @# ty) : Bool @# ty :=
-  (Switch val Of Bit 5 Retn Bool With {
-            $$ (natToWord 5 5) ::= $$ true ;
-            $$ (natToWord 5 6) ::= $$ false
-          })%kami_expr.
-
-
-Local Example test2 a b := (ConcatMod (test a) (test b))%kami.
-
-Definition extractArbitraryRange ty sz (inst: Bit sz ## ty) (range: nat * nat):
-  Bit (fst range + 1 - snd range) ## ty :=
-  (LETE i <- inst ;
-     RetE (ConstExtract (snd range) (fst range + 1 - snd range) (sz - 1 - fst range)
-                        (ZeroExtendTruncLsb _ #i)))%kami_expr.
-   
-
-Section unittests.
-
-  Open Scope kami_expr.
-
-  Local Notation "X ==> Y" := (evalExpr X = Y) (at level 75).
-
-  Let test_struct
-    :=  STRUCT {
-            "field0" ::= Const type false;
-            "field1" ::= Const type (natToWord 4 2);
-            "field2" ::= Const type (natToWord 5 3)}%kami_expr%struct_init.
-
-  Section struct_get_field_default_unittests.
-    Let test0
-    :  test_struct @% "field0" ==> false
-      := eq_refl false.
-
-    Let test1
-      : test_struct @% "field1" ==> natToWord 4 2
-      := eq_refl (natToWord 4 2).
-    
-    Let test2
-      : test_struct @% "field2" ==> natToWord 5 3
-      := eq_refl (natToWord 5 3).
-
-  End struct_get_field_default_unittests.
-
-  Section struct_set_field_unittests.
-
-    Let test_0
-    :  (test_struct @%["field0" <- (Const type true)]) @% "field0"
-                                                       ==> true
-      := eq_refl true.
-
-    Let test_1
-      :  (test_struct @%["field1" <- (Const type (natToWord 4 5))]) @% "field1"
-                                                                    ==> natToWord 4 5
-      := eq_refl (natToWord 4 5).
-
-    Let test_2
-      :  (test_struct @%["field2" <- (Const type (natToWord 5 5))]) @% "field2"
-                                                                    ==> natToWord 5 5
-      := eq_refl (natToWord 5 5).
-  End struct_set_field_unittests.
-
-  Close Scope kami_expr.
-
-End unittests.
-
-
-Local Definition testConcat ty (w1: Bit 10 @# ty) (w2: Bit 2 @# ty) (w3: Bit 5 @# ty) :=
-  {< w1, w2, w3 >}%kami_expr.
-
-Local Definition testArrayAccess ty (v: Array 4 (Bit 10) @# ty) (idx : Bit 2 @# ty) := (v @[ idx <- v @[ idx ]])%kami_expr.
-
-Local Definition testConstNat ty (w1 w2: Bit 10 @# ty): Bit 10 @# ty := (w1 + w2 + $4 + $6)%kami_expr.
-
-Local Definition testExtract ty n n1 n2 (pf1: n > n1) (pf2: n1 > n2) (a: Bit n @# ty) := (a $#[n1 : n2])%kami_expr.
-
-
-
-
-
-
-
-
-
-
-
-
-(* Useful Struct *)
-Definition Maybe k :=  STRUCT_TYPE {
-                           "valid" :: Bool;
-                           "data"  :: k }.
-
-Definition Pair (A B: Kind) := STRUCT_TYPE {
-                                   "fst" :: A;
-                                   "snd" :: B }.
-
-
-
-Definition Invalid {ty: Kind -> Type} {k} := (STRUCT { "valid" ::= $$ false ; "data" ::= $$ (getDefaultConst k) })%kami_expr.
-
-
-Local Definition testStruct :=
-  (STRUCT_TYPE {
-       "hello" :: Bit 10 ;
-       "a" :: Bit 3 ;
-       "b" :: Bit 5 ;
-       "test" :: Bool }).
-
-Local Definition testStructVal {ty}: testStruct @# ty :=
-  (STRUCT {
-       "hello" ::= $ 4 ;
-       "a" ::= $ 23 ;
-       "b" ::= $ 5 ;
-       "test" ::= $$ true })%kami_expr.
-
-
-
-Local Open Scope kami_action.
-Local Open Scope kami_expr.
-Local Definition testFieldAccess (ty: Kind -> Type): ActionT ty (Bit 10) :=
-  (LET val: testStruct <- testStructVal;
-     Ret (#val @% "hello"))%kami_action.
-Local Close Scope kami_expr.
-Local Close Scope kami_action.
-
-Local Definition testFieldUpd (ty: Kind -> Type) := 
-  ((testStructVal (ty := ty)) @%[ "hello" <- Const ty (natToWord 10 23) ])%kami_expr.
-
-
-
+(** * stuff to move elsewhere *)
+
+(* TODO: move to KamiStdLib? *)
+(* Definition extractArbitraryRange ty sz (inst: Bit sz ## ty) (range: nat * nat): *)
+(*   Bit (fst range + 1 - snd range) ## ty := *)
+(*   (LETE i <- inst ; *)
+(*      RetE (ConstExtract (snd range) (fst range + 1 - snd range) (sz - 1 - fst range) *)
+(*                         (ZeroExtendTruncLsb _ #i)))%kami_expr. *)
+Definition extractArbitraryRange ty sz (inst: LetExprSyntax ty (Bit sz)) (range: nat * nat): LetExprSyntax ty (Bit (Init.Nat.sub (Init.Nat.add (fst range) (S O)) (snd range))) :=
+  LetE inst
+       (fun i : ty (Bit sz) =>
+          NormExpr
+            (ConstExtract (snd range) (Init.Nat.sub (Init.Nat.add (fst range) (S O)) (snd range))
+                          (Init.Nat.sub (Init.Nat.sub sz (S O)) (fst range))
+                          (ZeroExtendTruncLsb
+                             (Init.Nat.add
+                                (Init.Nat.add (snd range) (Init.Nat.sub (Init.Nat.add (fst range) (S O)) (snd range)))
+                                (Init.Nat.sub (Init.Nat.sub sz (S O)) (fst range))) (Var ty (SyntaxKind (Bit sz)) i)))).
+
+(* Useful Struct:
+   TODO: move notation versions to StdLibKami*)
+(* Definition Maybe k :=  STRUCT_TYPE { *)
+(*                            "valid" :: Bool; *)
+(*                            "data"  :: k }. *)
+Definition Maybe k := getStruct [("valid", Bool);
+                                    ("data", k)].
+
+(* Definition Pair (A B: Kind) := STRUCT_TYPE { *)
+(*                                    "fst" :: A; *)
+(*                                    "snd" :: B }. *)
+Definition Pair (A B: Kind) := getStruct [("fst", A);
+                                            ("snd", B)].
+
+
+(* Definition Invalid {ty: Kind -> Type} {k} := (STRUCT { "valid" ::= $$ false ; "data" ::= $$ (getDefaultConst k) })%kami_expr. *)
+Definition Invalid {ty: Kind -> Type} {k} :=
+  BuildStruct
+  (fun
+     i : t
+           (Datatypes.length
+              (map (projT1 (P:=fun a : prod string Kind => Expr ty (SyntaxKind (snd a))))
+                 (cons
+                    (existT (fun a : prod string Kind => Expr ty (SyntaxKind (snd a)))
+                       (pair
+                          (String (Ascii false true true false true true true false)
+                             (String (Ascii true false false false false true true false)
+                                (String (Ascii false false true true false true true false)
+                                   (String (Ascii true false false true false true true false)
+                                      (String (Ascii false false true false false true true false) EmptyString))))) Bool)
+                       (Const ty false))
+                    (cons
+                       (existT (fun a : prod string Kind => Expr ty (SyntaxKind (snd a)))
+                          (pair
+                             (String (Ascii false false true false false true true false)
+                                (String (Ascii true false false false false true true false)
+                                   (String (Ascii false false true false true true true false)
+                                      (String (Ascii true false false false false true true false) EmptyString)))) k)
+                          (Const ty (getDefaultConst k))) nil)))) =>
+   snd
+     (nth_Fin
+        (map (projT1 (P:=fun a : prod string Kind => Expr ty (SyntaxKind (snd a))))
+           (cons
+              (existT (fun a : prod string Kind => Expr ty (SyntaxKind (snd a)))
+                 (pair
+                    (String (Ascii false true true false true true true false)
+                       (String (Ascii true false false false false true true false)
+                          (String (Ascii false false true true false true true false)
+                             (String (Ascii true false false true false true true false)
+                                (String (Ascii false false true false false true true false) EmptyString))))) Bool) 
+                 (Const ty false))
+              (cons
+                 (existT (fun a : prod string Kind => Expr ty (SyntaxKind (snd a)))
+                    (pair
+                       (String (Ascii false false true false false true true false)
+                          (String (Ascii true false false false false true true false)
+                             (String (Ascii false false true false true true true false)
+                                (String (Ascii true false false false false true true false) EmptyString)))) k)
+                    (Const ty (getDefaultConst k))) nil))) i))
+  (fun
+     j : t
+           (Datatypes.length
+              (map (projT1 (P:=fun a : prod string Kind => Expr ty (SyntaxKind (snd a))))
+                 (cons
+                    (existT (fun a : prod string Kind => Expr ty (SyntaxKind (snd a)))
+                       (pair
+                          (String (Ascii false true true false true true true false)
+                             (String (Ascii true false false false false true true false)
+                                (String (Ascii false false true true false true true false)
+                                   (String (Ascii true false false true false true true false)
+                                      (String (Ascii false false true false false true true false) EmptyString))))) Bool)
+                       (Const ty false))
+                    (cons
+                       (existT (fun a : prod string Kind => Expr ty (SyntaxKind (snd a)))
+                          (pair
+                             (String (Ascii false false true false false true true false)
+                                (String (Ascii true false false false false true true false)
+                                   (String (Ascii false false true false true true true false)
+                                      (String (Ascii true false false false false true true false) EmptyString)))) k)
+                          (Const ty (getDefaultConst k))) nil)))) =>
+   fst
+     (nth_Fin
+        (map (projT1 (P:=fun a : prod string Kind => Expr ty (SyntaxKind (snd a))))
+           (cons
+              (existT (fun a : prod string Kind => Expr ty (SyntaxKind (snd a)))
+                 (pair
+                    (String (Ascii false true true false true true true false)
+                       (String (Ascii true false false false false true true false)
+                          (String (Ascii false false true true false true true false)
+                             (String (Ascii true false false true false true true false)
+                                (String (Ascii false false true false false true true false) EmptyString))))) Bool) 
+                 (Const ty false))
+              (cons
+                 (existT (fun a : prod string Kind => Expr ty (SyntaxKind (snd a)))
+                    (pair
+                       (String (Ascii false false true false false true true false)
+                          (String (Ascii true false false false false true true false)
+                             (String (Ascii false false true false true true true false)
+                                (String (Ascii true false false false false true true false) EmptyString)))) k)
+                    (Const ty (getDefaultConst k))) nil))) j))
+  (fun
+     k0 : t
+            (Datatypes.length
+               (map (projT1 (P:=fun a : prod string Kind => Expr ty (SyntaxKind (snd a))))
+                  (cons
+                     (existT (fun a : prod string Kind => Expr ty (SyntaxKind (snd a)))
+                        (pair
+                           (String (Ascii false true true false true true true false)
+                              (String (Ascii true false false false false true true false)
+                                 (String (Ascii false false true true false true true false)
+                                    (String (Ascii true false false true false true true false)
+                                       (String (Ascii false false true false false true true false) EmptyString))))) Bool)
+                        (Const ty false))
+                     (cons
+                        (existT (fun a : prod string Kind => Expr ty (SyntaxKind (snd a)))
+                           (pair
+                              (String (Ascii false false true false false true true false)
+                                 (String (Ascii true false false false false true true false)
+                                    (String (Ascii false false true false true true true false)
+                                       (String (Ascii true false false false false true true false) EmptyString)))) k)
+                           (Const ty (getDefaultConst k))) nil)))) =>
+   nth_Fin_map2 (projT1 (P:=fun a : prod string Kind => Expr ty (SyntaxKind (snd a))))
+     (fun x : prod string Kind => Expr ty (SyntaxKind (snd x)))
+     (cons
+        (existT (fun a : prod string Kind => Expr ty (SyntaxKind (snd a)))
+           (pair
+              (String (Ascii false true true false true true true false)
+                 (String (Ascii true false false false false true true false)
+                    (String (Ascii false false true true false true true false)
+                       (String (Ascii true false false true false true true false)
+                          (String (Ascii false false true false false true true false) EmptyString))))) Bool) 
+           (Const ty false))
+        (cons
+           (existT (fun a : prod string Kind => Expr ty (SyntaxKind (snd a)))
+              (pair
+                 (String (Ascii false false true false false true true false)
+                    (String (Ascii true false false false false true true false)
+                       (String (Ascii false false true false true true true false)
+                          (String (Ascii true false false false false true true false) EmptyString)))) k) (Const ty (getDefaultConst k)))
+           nil)) k0
+     (projT2
+        (nth_Fin
+           (cons
+              (existT (fun a : prod string Kind => Expr ty (SyntaxKind (snd a)))
+                 (pair
+                    (String (Ascii false true true false true true true false)
+                       (String (Ascii true false false false false true true false)
+                          (String (Ascii false false true true false true true false)
+                             (String (Ascii true false false true false true true false)
+                                (String (Ascii false false true false false true true false) EmptyString))))) Bool) 
+                 (Const ty false))
+              (cons
+                 (existT (fun a : prod string Kind => Expr ty (SyntaxKind (snd a)))
+                    (pair
+                       (String (Ascii false false true false false true true false)
+                          (String (Ascii true false false false false true true false)
+                             (String (Ascii false false true false true true true false)
+                                (String (Ascii true false false false false true true false) EmptyString)))) k)
+                    (Const ty (getDefaultConst k))) nil))
+           (cast k0
+              (map_length_red (projT1 (P:=fun a : prod string Kind => Expr ty (SyntaxKind (snd a))))
+                 (cons
+                    (existT (fun a : prod string Kind => Expr ty (SyntaxKind (snd a)))
+                       (pair
+                          (String (Ascii false true true false true true true false)
+                             (String (Ascii true false false false false true true false)
+                                (String (Ascii false false true true false true true false)
+                                   (String (Ascii true false false true false true true false)
+                                      (String (Ascii false false true false false true true false) EmptyString))))) Bool)
+                       (Const ty false))
+                    (cons
+                       (existT (fun a : prod string Kind => Expr ty (SyntaxKind (snd a)))
+                          (pair
+                             (String (Ascii false false true false false true true false)
+                                (String (Ascii true false false false false true true false)
+                                   (String (Ascii false false true false true true true false)
+                                      (String (Ascii true false false false false true true false) EmptyString)))) k)
+                          (Const ty (getDefaultConst k))) nil))))))).
 (* TODO
    + Compiler verification (difficult)
    + PUAR: Linux/Certikos
  *)
-
