SyntaxDoubleWrites.v
@@ -1,8 +1,6 @@
 Require Export Bool Ascii String List FunctionalExtensionality Psatz PeanoNat.
 Require Export bbv.Word Lib.VectorFacts Lib.EclecticLib All.
 
-Require Kami.Syntax. Import KamiNotations.
-
 Export Word.Notations.
 
 Require Import Permutation RecordUpdate.RecordSet.
