Tests.v
@@ -1,0 +1,158 @@
+Require Import Syntax KamiNotations.
+Section mod_test.
+  Variable a: string.
+  Local Notation "^ x" := (a ++ "." ++ x)%string (at level 0).
+  Local Example test := MOD_WF{
+                              Register (^"x") : Bool <- true
+                                with Register (^"y") : Bool <- false
+                                with Rule (^"r1") := ( Read y: Bool <- ^"y";
+                                                         Write (^"x"): Bool <- #y;
+                                                         Retv )
+                          }.
+
+  Local Example test1 := MODULE_WF{
+                             Register (^"x") : Bool <- true
+                               with Register (^"y") : Bool <- false
+                               with Rule (^"r1") := ( Read y: Bool <- ^"y";
+                                                        Write (^"x"): Bool <- #y;
+                                                        Retv )
+                           }.
+End mod_test.
+
+
+
+
+
+Local Example test_normaldisj:
+  DisjKey (map (fun x => (x, 1)) ("a" :: "b" :: "c" :: nil))%string
+          (map (fun x => (x, 2)) ("d" :: "e" :: nil))%string.
+Proof.
+  simpl.
+  discharge_DisjKey.
+Qed.
+
+Local Example test_prefix_disj a:
+  DisjKey (map (fun x => ((a ++ x)%string, 1)) ("ab" :: "be" :: "cs" :: nil))%string
+          (map (fun x => ((a ++ x)%string, 2)) ("de" :: "et" :: nil))%string.
+Proof.
+  simpl.
+  discharge_DisjKey.
+Qed.
+
+Local Example test_suffix_disj a:
+  DisjKey (map (fun x => ((x ++ a)%string, 1)) ("ab" :: "be" :: "cs" :: nil))%string
+          (map (fun x => ((x ++ a)%string, 2)) ("de" :: "et" :: nil))%string.
+Proof.
+  simpl.
+  discharge_DisjKey.
+Qed.
+
+
+
+
+(* Testing the Notations *)
+
+Local Example testSwitch ty (val: Bit 5 @# ty) (a b: Bool @# ty) : Bool @# ty :=
+  (Switch val Retn Bool With {
+            $$ (natToWord 5 5) ::= $$ true ;
+            $$ (natToWord 5 6) ::= $$ false
+          })%kami_expr.
+
+Local Example testSwitch2 ty (val: Bit 5 @# ty) (a b: Bool @# ty) : Bool @# ty :=
+  (Switch val Of Bit 5 Retn Bool With {
+            $$ (natToWord 5 5) ::= $$ true ;
+            $$ (natToWord 5 6) ::= $$ false
+          })%kami_expr.
+
+
+Local Example test2 a b := (ConcatMod (test a) (test b))%kami.
+
+Section unittests.
+
+  Open Scope kami_expr.
+
+  Local Notation "X ==> Y" := (evalExpr X = Y) (at level 75).
+
+  Let test_struct
+    :=  STRUCT {
+            "field0" ::= Const type false;
+            "field1" ::= Const type (natToWord 4 2);
+            "field2" ::= Const type (natToWord 5 3)}%kami_expr%struct_init.
+
+  Section struct_get_field_default_unittests.
+    Let test0
+    :  test_struct @% "field0" ==> false
+      := eq_refl false.
+
+    Let test1
+      : test_struct @% "field1" ==> natToWord 4 2
+      := eq_refl (natToWord 4 2).
+    
+    Let test2
+      : test_struct @% "field2" ==> natToWord 5 3
+      := eq_refl (natToWord 5 3).
+
+  End struct_get_field_default_unittests.
+
+  Section struct_set_field_unittests.
+
+    Let test_0
+    :  (test_struct @%["field0" <- (Const type true)]) @% "field0"
+                                                       ==> true
+      := eq_refl true.
+
+    Let test_1
+      :  (test_struct @%["field1" <- (Const type (natToWord 4 5))]) @% "field1"
+                                                                    ==> natToWord 4 5
+      := eq_refl (natToWord 4 5).
+
+    Let test_2
+      :  (test_struct @%["field2" <- (Const type (natToWord 5 5))]) @% "field2"
+                                                                    ==> natToWord 5 5
+      := eq_refl (natToWord 5 5).
+  End struct_set_field_unittests.
+
+  Close Scope kami_expr.
+
+End unittests.
+
+
+Local Definition testConcat ty (w1: Bit 10 @# ty) (w2: Bit 2 @# ty) (w3: Bit 5 @# ty) :=
+  {< w1, w2, w3 >}%kami_expr.
+
+Local Definition testArrayAccess ty (v: Array 4 (Bit 10) @# ty) (idx : Bit 2 @# ty) := (v @[ idx <- v @[ idx ]])%kami_expr.
+
+Local Definition testConstNat ty (w1 w2: Bit 10 @# ty): Bit 10 @# ty := (w1 + w2 + $4 + $6)%kami_expr.
+
+Local Definition testExtract ty n n1 n2 (pf1: n > n1) (pf2: n1 > n2) (a: Bit n @# ty) := (a $#[n1 : n2])%kami_expr.
+
+
+
+
+
+Local Definition testStruct :=
+  (STRUCT_TYPE {
+       "hello" :: Bit 10 ;
+       "a" :: Bit 3 ;
+       "b" :: Bit 5 ;
+       "test" :: Bool }).
+
+Local Definition testStructVal {ty}: testStruct @# ty :=
+  (STRUCT {
+       "hello" ::= $ 4 ;
+       "a" ::= $ 23 ;
+       "b" ::= $ 5 ;
+       "test" ::= $$ true })%kami_expr.
+
+
+
+Local Open Scope kami_action.
+Local Open Scope kami_expr.
+Local Definition testFieldAccess (ty: Kind -> Type): ActionT ty (Bit 10) :=
+  (LET val: testStruct <- testStructVal;
+     Ret (#val @% "hello"))%kami_action.
+Local Close Scope kami_expr.
+Local Close Scope kami_action.
+
+Local Definition testFieldUpd (ty: Kind -> Type) := 
+  ((testStructVal (ty := ty)) @%[ "hello" <- Const ty (natToWord 10 23) ])%kami_expr.
